In progress updates

high/Veritas.Verifier.Blum.fsti
@@ -31,36 +31,42 @@ let ts_add_set (ep: epoch) (itsl: its_log): mset_ms_hashfn_dom
 
 val lemma_add_elem_correct (itsl: its_log) (i: I.seq_index itsl):
   Lemma (requires (is_blum_add (I.index itsl i)))
-        (ensures (let ep = TL.epoch_of itsl i in
-                  ts_add_set ep itsl `contains` blum_add_elem (I.index itsl i)))
+        (ensures (let e = I.index itsl i in
+                  let be = blum_add_elem e in
+                  let ep = MH.epoch_of be in
+                  ts_add_set ep itsl `contains` be))
 
 (* sequence of blum adds in epoch ep restricted to key k *)
 val ts_add_seq_key (ep: epoch) (itsl: its_log) (k:key): seq ms_hashfn_dom
 
 (* the addset restricted to key k *)
-let ts_add_set_key (itsl: its_log) (k:key): mset_ms_hashfn_dom
-  = seq2mset #_ #ms_hashfn_dom_cmp (ts_add_seq_key itsl k)
+let ts_add_set_key (ep: epoch) (itsl: its_log) (k:key): mset_ms_hashfn_dom
+  = seq2mset #_ #ms_hashfn_dom_cmp (ts_add_seq_key ep itsl k)
 
 (* the blum adds in the time sequenced log should be the same as global add set *)
-val lemma_ts_add_set_correct (itsl: its_log): 
-  Lemma (ts_add_set itsl == g_add_set (g_vlog_of itsl))
+val lemma_ts_add_set_correct (ep: epoch) (itsl: its_log):
+  Lemma (ts_add_set ep itsl == g_add_set ep (g_vlog_of itsl))
 
 (* if the tail element is a blum add, then the add set is obtained by adding that 
  * blum add to the prefix *)
 val lemma_ts_add_set_key_extend (itsl: its_log {I.length itsl > 0}):
   Lemma (requires (is_blum_add (I.telem itsl)))
-        (ensures (ts_add_set_key itsl (key_of (I.index itsl (I.length itsl - 1))) == 
-                  add_elem (ts_add_set_key (I.prefix itsl (I.length itsl - 1))
-                                           (key_of (I.index itsl (I.length itsl - 1))))
-                           (blum_add_elem (I.telem itsl))))
+        (ensures (let e = I.telem itsl in
+                  let k = key_of e in
+                  let be = blum_add_elem e in
+                  let ep = MH.epoch_of be in
+                  let n = I.length itsl in
+                  let itsl' = I.prefix itsl (n - 1) in
+                  ts_add_set_key ep itsl k ==
+                  add_elem (ts_add_set_key ep itsl' k) be))
 
-val some_add_elem_idx (itsl: its_log) 
-  (be: ms_hashfn_dom{ts_add_set itsl `MS.contains` be}): 
+val some_add_elem_idx (ep: epoch) (itsl: its_log)
+  (be: ms_hashfn_dom{ts_add_set ep itsl `MS.contains` be}):
   (i:(I.seq_index itsl){is_blum_add (I.index itsl i) /\
                       be = blum_add_elem (I.index itsl i)})
 
-val lemma_ts_add_set_key_contains_only (itsl: its_log) (k:key) (be: ms_hashfn_dom):
-  Lemma (requires (ts_add_set_key itsl k `MS.contains` be))
+val lemma_ts_add_set_key_contains_only (ep: epoch) (itsl: its_log) (k:key) (be: ms_hashfn_dom):
+  Lemma (requires (ts_add_set_key ep itsl k `MS.contains` be))
         (ensures (MH.key_of be = k))
 
 (* get the blum evict element from an index *)
@@ -72,51 +78,57 @@ val lemma_index_blum_evict_prefix (itsl: its_log) (i:nat{i <= I.length itsl}) (j
         (ensures (blum_evict_elem itsl j = blum_evict_elem (I.prefix itsl i) j))
         [SMTPat (blum_evict_elem (I.prefix itsl i) j)]
 
-
 (* sequence of evicts in time sequence log *)
-val ts_evict_seq (itsl: its_log): seq ms_hashfn_dom
+val ts_evict_seq (ep: epoch) (itsl: its_log): seq ms_hashfn_dom
 
 (* set of evicts in time sequence log *)
-let ts_evict_set (itsl: its_log): mset_ms_hashfn_dom = 
-  seq2mset #_ #ms_hashfn_dom_cmp (ts_evict_seq itsl)
+let ts_evict_set (ep: epoch) (itsl: its_log): mset_ms_hashfn_dom =
+  seq2mset #_ #ms_hashfn_dom_cmp (ts_evict_seq ep itsl)
 
 (* the evict sequence restricted to key k *)
-val ts_evict_seq_key (itsl: its_log) (k:key): seq ms_hashfn_dom
+val ts_evict_seq_key (ep: epoch) (itsl: its_log) (k:key): seq ms_hashfn_dom
 
-let ts_evict_set_key (itsl: its_log) (k:key): mset_ms_hashfn_dom= 
-  seq2mset #_ #ms_hashfn_dom_cmp (ts_evict_seq_key itsl k)
+let ts_evict_set_key (ep: epoch) (itsl: its_log) (k:key): mset_ms_hashfn_dom=
+  seq2mset #_ #ms_hashfn_dom_cmp (ts_evict_seq_key ep itsl k)
 
 (* the blum evicts in time sequenced log should be the same as global evict set *)
-val lemma_ts_evict_set_correct (itsl: its_log):
-  Lemma (ts_evict_set itsl == g_evict_set (g_vlog_of itsl))
+val lemma_ts_evict_set_correct (ep: epoch) (itsl: its_log):
+  Lemma (ts_evict_set ep itsl == g_evict_set ep (g_vlog_of itsl))
 
 (* if the tail element is not an evict, the evict set is the same as the evict 
  * set of the length - 1 prefix 
  *)
-val lemma_ts_evict_set_key_extend2 (itsl: its_log {I.length itsl > 0}):
+val lemma_ts_evict_set_key_extend2 (ep: epoch) (itsl: its_log {I.length itsl > 0}):
   Lemma (requires (not (is_evict_to_blum (I.index itsl (I.length itsl - 1)))))
-        (ensures (ts_evict_set_key itsl (key_of (I.index itsl (I.length itsl - 1))) == 
-                  ts_evict_set_key (I.prefix itsl (I.length itsl - 1))
-                                           (key_of (I.index itsl (I.length itsl - 1)))))
+        (ensures (let n = I.length itsl in
+                  let itsl' = I.prefix itsl (n - 1) in
+                  let e = I.index itsl (n - 1) in
+                  let k = key_of e in
+                  ts_evict_set_key ep itsl k ==
+                  ts_evict_set_key ep itsl' k))
 
 (* since evict_set is a pure set (not a multiset) we can identify the unique index 
  * for each element of the set *)
-val index_blum_evict (itsl: its_log) (e: ms_hashfn_dom {ts_evict_set itsl `contains` e}):
+val index_blum_evict (ep: epoch) (itsl: its_log) (e: ms_hashfn_dom {ts_evict_set ep itsl `contains` e}):
   (i:I.seq_index itsl{is_evict_to_blum (I.index itsl i) /\ 
                     blum_evict_elem itsl i = e})
 
 (* if the blum add occurs in the blum evict set, its index is earlier *)
 val lemma_evict_before_add (itsl: its_log) (i:I.seq_index itsl{is_blum_add (I.index itsl i)}):
-  Lemma (requires True)
-        (ensures (not (ts_evict_set itsl `contains` blum_add_elem (I.index itsl i)) \/
-                  index_blum_evict itsl (blum_add_elem (I.index itsl i)) < i))
+  Lemma (ensures (let e = I.index itsl i in
+                  let be = blum_add_elem e in
+                  let ep = MH.epoch_of be in
+                  not (ts_evict_set ep itsl `contains` be) \/
+                  index_blum_evict ep itsl be < i))
 
 (* a slightly different version of of the previous lemma - the count of an add element 
  * in the evict set is the same in the prefix as the full sequence *)
 val lemma_evict_before_add2 (itsl: its_log) (i:I.seq_index itsl{is_blum_add (I.index itsl i)}):
-   Lemma (requires True)
-         (ensures (MS.mem (blum_add_elem (I.index itsl i)) (ts_evict_set itsl) =
-                   MS.mem (blum_add_elem (I.index itsl i)) (ts_evict_set (I.prefix itsl i))))
+   Lemma (ensures (let e = I.index itsl i in
+                   let be = blum_add_elem e in
+                   let ep = MH.epoch_of be in
+                   MS.mem be (ts_evict_set ep itsl) =
+                   MS.mem be (ts_evict_set ep (I.prefix itsl i))))
 
 val lemma_evict_before_add3 (itsl: its_log) (i: I.seq_index itsl) (j:I.seq_index itsl):
   Lemma (requires (is_blum_add (I.index itsl i) /\
@@ -125,27 +137,27 @@ val lemma_evict_before_add3 (itsl: its_log) (i: I.seq_index itsl) (j:I.seq_index
         (ensures (j < i))
 
 (* for an eac ts log, if the eac state of a key k is instore, the count of blum evicts 
- * is the same of blum adds for that key *)
-val lemma_evict_add_count_same (itsl: TL.eac_log) (k:key):
+ * is the same of blum adds for that key for any epoch *)
+val lemma_evict_add_count_same (ep: epoch) (itsl: TL.eac_log) (k:key):
   Lemma (requires (TL.is_eac_state_instore itsl k))
-        (ensures (MS.size (ts_add_set_key itsl k) = MS.size (ts_evict_set_key itsl k)))
+        (ensures (MS.size (ts_add_set_key ep itsl k) = MS.size (ts_evict_set_key ep itsl k)))
 
 (* for an eac ts log, if the eac state of a key k is evicted to merkle, the count of blum evicts 
  * is the same of blum adds for that key *)
-val lemma_evict_add_count_same_evictedm (itsl: TL.eac_log) (k:key):
+val lemma_evict_add_count_same_evictedm (ep: epoch) (itsl: TL.eac_log) (k:key):
   Lemma (requires (is_eac_state_evicted_merkle itsl k))
-        (ensures (MS.size (ts_add_set_key itsl k) = MS.size (ts_evict_set_key itsl k)))
+        (ensures (MS.size (ts_add_set_key ep itsl k) = MS.size (ts_evict_set_key ep itsl k)))
 
-val lemma_mem_key_add_set_same (itsl: its_log) (be: ms_hashfn_dom):
-  Lemma (mem be (ts_add_set itsl) = mem be (ts_add_set_key itsl (MH.key_of be)))
+val lemma_mem_key_add_set_same (ep: epoch) (itsl: its_log) (be: ms_hashfn_dom):
+  Lemma (mem be (ts_add_set ep itsl) = mem be (ts_add_set_key ep itsl (MH.key_of be)))
 
-val lemma_mem_key_evict_set_same (itsl: its_log) (be: ms_hashfn_dom):
-  Lemma (mem be (ts_evict_set itsl) = mem be (ts_evict_set_key itsl (MH.key_of be)))
+val lemma_mem_key_evict_set_same (ep: epoch) (itsl: its_log) (be: ms_hashfn_dom):
+  Lemma (mem be (ts_evict_set ep itsl) = mem be (ts_evict_set_key ep itsl (MH.key_of be)))
 
 (* the count of an element can only decrease in a prefix of itsl *)
-val lemma_mem_monotonic (be:ms_hashfn_dom) (itsl: its_log) (i:nat{i <= I.length itsl}):
-  Lemma (mem be (ts_evict_set itsl) >= mem be (ts_evict_set (I.prefix itsl i)) /\
-         mem be (ts_add_set itsl) >= mem be (ts_add_set (I.prefix itsl i)))
+val lemma_mem_monotonic (ep: epoch) (be:ms_hashfn_dom) (itsl: its_log) (i:nat{i <= I.length itsl}):
+  Lemma (mem be (ts_evict_set ep itsl) >= mem be (ts_evict_set ep (I.prefix itsl i)) /\
+         mem be (ts_add_set ep itsl) >= mem be (ts_add_set ep (I.prefix itsl i)))
 
 (* the next add of a blum evict is a blum add of the same "element" *)
 val lemma_blum_evict_add_same (itsl: TL.eac_log) (i:I.seq_index itsl):
@@ -173,7 +185,9 @@ val lemma_add_set_mem (itsl: its_log) (i: I.seq_index itsl) (j:I.seq_index itsl{
   Lemma (requires (is_blum_add (I.index itsl i) /\
                    is_blum_add (I.index itsl j) /\
                    blum_add_elem (I.index itsl i) = blum_add_elem (I.index itsl j)))
-        (ensures (MS.mem (blum_add_elem (I.index itsl i)) (ts_add_set itsl) >= 2))
+        (ensures (let be = blum_add_elem (I.index itsl i) in
+                  let ep = MH.epoch_of be in
+                  MS.mem (blum_add_elem (I.index itsl i)) (ts_add_set ep itsl) >= 2))
 
 val eac_instore_addb_diff_elem (itsl: its_log) 
                                (i: I.seq_index itsl{let itsli = I.prefix itsl i in
