high/Veritas.Verifier.Global.fsti
@@ -90,11 +90,6 @@ let clock (gl: verifiable_log) (i: sseq_index gl): timestamp =
   let tl = thread_log gl tid in
   VT.clock tl idx
 
-let epoch_of (gl: verifiable_log) (i: sseq_index gl): epoch =
-  let (tid, idx) = i in
-  let tl = thread_log gl tid in
-  VT.epoch_of tl idx
-
 (* global add sequence *)
 val g_add_seq (ep: epoch) (gl: verifiable_log): seq (ms_hashfn_dom)
 
@@ -106,37 +101,44 @@ let g_add_set (ep: epoch) (gl: verifiable_log): mset_ms_hashfn_dom =
 val lemma_g_hadd_correct (ep: epoch) (gl: verifiable_log):
   Lemma (hadd gl ep = ms_hashfn (g_add_seq ep gl))
 
-(* mapping from blum_add entries in verifier log to the index in add seq *)
+(* mapping from blum_add entries in verifier log to the index in add seq of the epoch *)
 val add_set_map (gl: verifiable_log) (ii: sseq_index gl {is_blum_add (indexss gl ii)}):
-  (
-
-  j: seq_index (g_add_seq gl){index (g_add_seq gl) j = blum_add_elem (indexss gl ii)})
+  (let e = indexss gl ii in
+   let be = blum_add_elem e in
+   let ep = epoch_of be in
+   let add_seq = g_add_seq ep gl in
+   j: seq_index add_seq {index add_seq j = be})
 
 (* inverse mapping from add_seq to the blum add entries in the verifier logs *)
-val add_set_map_inv (gl: verifiable_log) (j: seq_index (g_add_seq gl)):
-  (ii: sseq_index gl {is_blum_add (indexss gl ii) /\ 
-                      add_set_map gl ii = j})
+val add_set_map_inv (ep: epoch) (gl: verifiable_log) (j: seq_index (g_add_seq ep gl)):
+  (ii: sseq_index gl {let e = indexss gl ii in
+                      is_blum_add e /\
+                      (let be = blum_add_elem e in
+                       let add_seq = g_add_seq ep gl in
+                       be = index add_seq j /\
+                       add_set_map gl ii = j /\
+                       ep = epoch_of be)})
 
 val lemma_add_set_map_inv (gl: verifiable_log)(ii: sseq_index gl {is_blum_add (indexss gl ii)}):
-  Lemma (requires True)
-        (ensures (add_set_map_inv gl (add_set_map gl ii) = ii))
+  Lemma (ensures (let e = indexss gl ii in
+                  let be = blum_add_elem e in
+                  let ep = epoch_of be in
+                  let j = add_set_map gl ii in
+                  add_set_map_inv ep gl j = ii))
         [SMTPat (add_set_map gl ii)]
 
 (* a single sequence containing all the blum evicts *)
-val g_evict_seq (gl: verifiable_log): seq ms_hashfn_dom 
+val g_evict_seq (ep: epoch) (gl: verifiable_log): seq ms_hashfn_dom
 
-(* sequence of blum evicts restricted to an epoch *)
-val g_evict_seq_epoch (gl: verifiable_log) (ep: epoch): seq ms_hashfn_dom
-
-let g_evict_set (gl: verifiable_log): mset_ms_hashfn_dom = 
-  seq2mset #_ #ms_hashfn_dom_cmp (g_evict_seq gl)
+let g_evict_set (ep: epoch) (gl: verifiable_log): mset_ms_hashfn_dom =
+  seq2mset #_ #ms_hashfn_dom_cmp (g_evict_seq ep gl)
 
 val lemma_ghevict_correct (gl: verifiable_log) (ep: epoch):
-  Lemma (hevict gl ep = ms_hashfn (g_evict_seq_epoch gl ep))
+  Lemma (hevict gl ep = ms_hashfn (g_evict_seq ep gl))
 
 (* the global evict set is a set (not a multiset) *)
-val g_evict_set_is_set (gl: verifiable_log): 
-  Lemma (is_set (g_evict_set gl))
+val g_evict_set_is_set (ep: epoch) (gl: verifiable_log):
+  Lemma (is_set (g_evict_set ep gl))
 
 let blum_evict_elem (gl: verifiable_log) (ii: sseq_index gl {is_evict_to_blum (indexss gl ii)}):
   ms_hashfn_dom = 
@@ -145,15 +147,26 @@ let blum_evict_elem (gl: verifiable_log) (ii: sseq_index gl {is_evict_to_blum (i
   VT.blum_evict_elem tl i
 
 val evict_seq_map (gl: verifiable_log) (ii: sseq_index gl {is_evict_to_blum (indexss gl ii)}):
-  (j: seq_index (g_evict_seq gl) {index (g_evict_seq gl) j = 
-                                  blum_evict_elem gl ii})
+  (let e = indexss gl ii in
+   let be = blum_evict_elem gl ii in
+   let ep = epoch_of be in
+   let evict_seq = g_evict_seq ep gl in
 
-val evict_seq_map_inv (gl: verifiable_log) (j: seq_index (g_evict_seq gl)):
-  (ii: sseq_index gl {is_evict_to_blum (indexss gl ii) /\
-                      blum_evict_elem gl ii = index (g_evict_seq gl) j /\
-                      evict_seq_map gl ii = j})
+   j: seq_index evict_seq {index evict_seq j = be})
+
+val evict_seq_map_inv (ep: epoch) (gl: verifiable_log) (j: seq_index (g_evict_seq ep gl)):
+  (ii: sseq_index gl {let e = indexss gl ii in
+                      is_evict_to_blum e /\
+                      (let be = blum_evict_elem gl ii in
+                       let evict_seq = g_evict_seq ep gl in
+                       be = index evict_seq j /\
+                       evict_seq_map gl ii = j /\
+                       ep = epoch_of be)})
 
 val lemma_evict_seq_inv (gl: verifiable_log) (ii: sseq_index gl {is_evict_to_blum (indexss gl ii)}):
-  Lemma (requires True)
-        (ensures (evict_seq_map_inv gl (evict_seq_map gl ii) = ii))
+  Lemma (ensures (let e = indexss gl ii in
+                  let be = blum_evict_elem gl ii in
+                  let ep = epoch_of be in
+                  let j = evict_seq_map gl ii in
+                  evict_seq_map_inv ep gl j = ii))
         [SMTPat (evict_seq_map gl ii)]
